Tried a few things.

CaseStudies/ABP/Sender_DS.thy
@@ -47,4 +47,42 @@ fixrec tsSnd_h :: "'a tstream \<rightarrow> bool tstream \<rightarrow> bool disc
 definition tsSnd :: "'a tstream \<rightarrow> bool tstream \<rightarrow> ('a \<times> bool) tstream" where
 "tsSnd \<equiv> \<Lambda> msg acks. delay (tsSnd_h\<cdot>msg\<cdot>acks\<cdot>(Discr True))"
 
+(*
+text {* input: msg from the user, acks from the receiver, ack buffer for the expected ack 
+        output: msg and expected ack for the receiver *}
+fixrec tsSnd_h :: "'a tstream \<rightarrow> bool tstream \<rightarrow> bool discr \<rightarrow> nat discr \<rightarrow> ('a \<times> bool) tstream" where
+  (* bottom case *)
+"tsSnd_h\<cdot>\<bottom>\<cdot>acks\<cdot>ack\<cdot>cou = \<bottom>" |
+"tsSnd_h\<cdot>msg\<cdot>\<bottom>\<cdot>ack\<cdot>cou = \<bottom>" |
+
+  (* if an input and ack from the receiver *)
+"msg \<noteq> \<bottom> \<Longrightarrow> acks \<noteq> \<bottom> \<Longrightarrow> tsSnd_h\<cdot>(tsLscons\<cdot>(up\<cdot>(uMsg\<cdot>m))\<cdot>msg)\<cdot>(tsLscons\<cdot>(up\<cdot>(uMsg\<cdot>a))\<cdot>acks)\<cdot>ack\<cdot>cou = 
+  (* ack for the current msg \<Longrightarrow> send next msg *)
+  (if (a = ack) then tsSnd_h\<cdot>msg\<cdot>acks\<cdot>(Discr (\<not>(undiscr ack)))\<cdot>cou
+  (* wrong ack for the current msg \<Longrightarrow> send msg again *)
+   else tsMLscons\<cdot>(upApply2 Pair\<cdot>(up\<cdot>m)\<cdot>(up\<cdot>ack))\<cdot>(tsSnd_h\<cdot>(tsMLscons\<cdot>(up\<cdot>m)\<cdot>msg)\<cdot>acks\<cdot>ack\<cdot>cou))" | 
+
+  (* if an input and ack is a tick \<Longrightarrow> send msg again plus a tick
+     if transmission starts with tick \<Longrightarrow> #\<surd> acks = \<infinity> *)
+"msg \<noteq> \<bottom> \<Longrightarrow> tsSnd_h\<cdot>(tsLscons\<cdot>(up\<cdot>(uMsg\<cdot>m))\<cdot>msg)\<cdot>(tsLscons\<cdot>(up\<cdot>DiscrTick)\<cdot>acks)\<cdot>ack\<cdot>cou  = 
+  (if (cou = Discr 0) then delayFun\<cdot>(tsSnd_h\<cdot>(tsMLscons\<cdot>(up\<cdot>m)\<cdot>msg)\<cdot>acks\<cdot>ack\<cdot>(Discr 1))
+   else tsMLscons\<cdot>(upApply2 Pair\<cdot>(up\<cdot>m)\<cdot>(up\<cdot>ack))\<cdot>(delayFun\<cdot>(tsSnd_h\<cdot>(tsMLscons\<cdot>(up\<cdot>m)\<cdot>msg)\<cdot>acks\<cdot>ack\<cdot>(Discr ((undiscr cou) - 1)))))" |
+
+  (* if input is a tick \<Longrightarrow> send tick and remove wrong ack *)
+"acks \<noteq> \<bottom> \<Longrightarrow> tsSnd_h\<cdot>(tsLscons\<cdot>(up\<cdot>DiscrTick)\<cdot>msg)\<cdot>(tsLscons\<cdot>(up\<cdot>(uMsg\<cdot>a))\<cdot>acks)\<cdot>ack\<cdot>cou
+  = delayFun\<cdot>(tsSnd_h\<cdot>msg\<cdot>acks\<cdot>ack\<cdot>cou)"
+
+definition tsSnd :: "'a tstream \<rightarrow> bool tstream \<rightarrow> ('a \<times> bool) tstream" where
+"tsSnd \<equiv> \<Lambda> msg acks. delay (tsSnd_h\<cdot>msg\<cdot>acks\<cdot>(Discr True)\<cdot>(Discr 1))"
+
+lemma tssnd_insert: "tsSnd\<cdot>msg\<cdot>acks = delay (tsSnd_h\<cdot>msg\<cdot>acks\<cdot>(Discr True)\<cdot>(Discr 1))"
+  by (simp add: tsSnd_def)
+
+lemma tssnd_h_strict [simp]:
+"tsSnd_h\<cdot>\<bottom>\<cdot>\<bottom>\<cdot>ack\<cdot>cou = \<bottom>"
+"tsSnd_h\<cdot>\<bottom>\<cdot>acks\<cdot>ack\<cdot>cou = \<bottom>"
+"tsSnd_h\<cdot>msg\<cdot>\<bottom>\<cdot>ack\<cdot>cou = \<bottom>"
+  by (fixrec_simp)+
+*)
+
 end
